properties for fragments

coq/Fragment.v
@@ -1,6 +1,6 @@
 
 
-Require Import Word NArith.
+Require Import NArith Word.
 Require ContractSem.
 
 Module Fragment (W:Word).
@@ -23,9 +23,7 @@ Fixpoint fragment_sem (exit_point:_ -> bool) (v : variable_env) (c :constant_env
   match steps with
     | O => FragmentStepRunOut
     | S remaining_steps =>
-      if exit_point v then
-        FragmentContinue v 
-      else
+      if exit_point v then FragmentContinue v else
       match v.(venv_prg_sfx) with
       | nil => FragmentToWorld ContractFail v.(venv_storage_at_call) v.(venv_balance_at_call) None
       | i :: _ =>
@@ -44,5 +42,178 @@ Fixpoint fragment_sem (exit_point:_ -> bool) (v : variable_env) (c :constant_env
       end
   end.
 
+Require Import List.
+
+
+Fixpoint program_length lst := match lst with
+ | nil => 0
+ | PUSH1 _ :: tl => 2 + program_length tl
+ | PUSH2 _ :: tl => 3 + program_length tl
+ | _ :: tl => 1 + program_length tl
+end.
+
+Definition in_loc v c loc :=
+  N.eqb (N_of_word loc + program_length v.(venv_prg_sfx))
+          (program_length c.(cenv_program)).
+
+Definition not_in_range loc n m := n < N_of_word loc \/ m > N_of_word loc.
+
+Definition pc v := program_length v.(venv_prg_sfx).
+
+Definition fragment_range c loc n m :=
+  forall v, n <= pc v <= m -> in_loc v c loc = false.
+
+Require Import Omega.
+
+Axiom zero_is_zero : word_iszero word_zero = true.
+
+Axiom word_mod_small : forall large small, N_of_word small < large ->
+  word_mod small (word_of_N large) = small.
+
+Definition is_jumpdest c loc := exists code,
+  N.eqb (N_of_word loc + program_length (JUMPDEST::code))
+          (program_length c.(cenv_program)) = true /\
+  drop_bytes (cenv_program c) (N_of_word (word_mod loc (word_of_N 256))) =
+  JUMPDEST :: code.
+
+Lemma program_length_app : forall c1 c2,
+  program_length c1 + program_length c2 = program_length (c1 ++ c2).
+induction c1.
+auto.
+intros.
+destruct a; rewrite <- app_comm_cons; unfold program_length; fold program_length; rewrite <- IHc1; ring.
+Qed.
+
+Lemma code_length : forall v code loc1 loc2,
+  v.(venv_prg_sfx) = PUSH1 loc1 :: JUMPI :: PUSH1 loc2 :: JUMP :: code ->
+  pc v - 6 = program_length code.
+intros.
+
+unfold pc.
+destruct v.
+unfold venv_prg_sfx.
+unfold venv_prg_sfx in H.
+rewrite H.
+unfold program_length.
+fold program_length.
+assert (2 + (1 + (2 + (1 + program_length code))) = program_length code + 6).
+ring.
+rewrite H0.
+rewrite N.add_sub.
+trivial.
+Qed.
+
+Lemma code_length2 : forall v code loc1 loc2,
+  v.(venv_prg_sfx) = PUSH1 loc1 :: JUMPI :: PUSH1 loc2 :: JUMP :: code ->
+  pc v = program_length code + 6.
+intros.
+
+unfold pc.
+destruct v.
+unfold venv_prg_sfx.
+unfold venv_prg_sfx in H.
+rewrite H.
+unfold program_length.
+fold program_length.
+ring.
+Qed.
+
+Lemma code_in_fragment : forall code frag len,
+  program_length frag <= len ->
+  program_length code <= program_length (frag ++ code) <= program_length code + len.
+intros.
+rewrite <- program_length_app.
+split.
+rewrite N.add_comm.
+apply N.le_add_r.
+rewrite N.add_comm.
+apply N.add_le_mono_l.
+trivial.
+Qed.
+
+Lemma pc_in_range : forall v v2 code loc1 loc2 frag,
+  v.(venv_prg_sfx) = PUSH1 loc1 :: JUMPI :: PUSH1 loc2 :: JUMP :: code ->
+  v2.(venv_prg_sfx) = frag ++ code ->
+  program_length frag <= 6 ->
+  pc v - 6 <= pc v2 <= pc v.
+intros.
+rewrite (code_length v code loc1 loc2); auto.
+rewrite (code_length2 v code loc1 loc2); auto.
+unfold pc.
+rewrite H0.
+apply code_in_fragment.
+auto.
+Qed.
+
+Lemma split_paths1 : forall v c loc1 loc2 code stack,
+  v.(venv_prg_sfx) = PUSH1 loc1 :: JUMPI :: PUSH1 loc2 :: JUMP :: code ->
+  v.(venv_stack) = word_zero :: stack ->
+  fragment_range c loc1 (pc v - 6) (pc v) ->
+  fragment_range c loc2 (pc v - 6) (pc v) ->
+  is_jumpdest c loc1 ->
+  is_jumpdest c loc2 ->
+  N_of_word loc1 < 256 ->
+  N_of_word loc2 < 256 ->
+  fragment_sem (fun v => orb (in_loc v c loc1) (in_loc v c loc2)) v c 5%nat =
+  FragmentContinue (venv_pop_stack 1%nat (venv_change_sfx (N_of_word loc2) v c)).
+intros.
+simpl.
+rewrite H1.
+rewrite H2.
+simpl.
+rewrite H; simpl.
+rewrite H1.
+rewrite H2; simpl.
+rewrite H; simpl.
+rewrite H0; simpl.
+
+rewrite zero_is_zero;simpl.
+rewrite H1.
+rewrite H2; simpl.
+rewrite H1.
+rewrite H2; simpl.
+elim H4;intros.
+elim H7; clear H7; intros.
+rewrite H8;simpl.
+unfold in_loc.
+unfold venv_prg_sfx.
+rewrite H7.
+rewrite Bool.orb_true_r.
+simpl.
+cbn.
+rewrite word_mod_small in H8.
+rewrite H8.
+auto.
+auto.
+
+apply (pc_in_range _ _ code loc1 loc2 (JUMP::nil));auto.
+apply N.leb_le;auto.
+
+apply (pc_in_range _ _ code loc1 loc2 (JUMP::nil));auto.
+apply N.leb_le;auto.
+
+apply (pc_in_range _ _ code loc1 loc2 (PUSH1 loc2 :: JUMP :: nil));auto.
+apply N.leb_le;auto.
+
+apply (pc_in_range _ _ code loc1 loc2 (PUSH1 loc2 :: JUMP :: nil));auto.
+apply N.leb_le;auto.
+
+rewrite H.
+
+apply (pc_in_range _ _ code loc1 loc2 (JUMPI::PUSH1 loc2 :: JUMP :: nil));auto.
+apply N.leb_le;auto.
+
+rewrite H.
+
+apply (pc_in_range _ _ code loc1 loc2 (JUMPI::PUSH1 loc2 :: JUMP :: nil));auto.
+apply N.leb_le;auto.
+
+apply (pc_in_range _ _ code loc1 loc2 (PUSH1 loc1::JUMPI::PUSH1 loc2 :: JUMP :: nil));auto.
+apply N.leb_le;auto.
+
+apply (pc_in_range _ _ code loc1 loc2 (PUSH1 loc1::JUMPI::PUSH1 loc2 :: JUMP :: nil));auto.
+apply N.leb_le;auto.
+
+Qed.
 End Fragment.
 
